Simplify more globals and package initialization

new/golang/defn/pkg.v
@@ -1,5 +1,5 @@
-From Perennial.goose_lang Require Import notation.
-From New.golang.defn Require Export typing.
+From New.golang.defn Require Import mem typing list assume.
+From Perennial Require Import base.
 
 (** [PkgInfo] associates a pkg_name to its static information. *)
 Class PkgInfo (pkg_name: go_string) `{ffi_syntax} := {
@@ -13,3 +13,79 @@ Arguments pkg_vars (pkg_name) {_ _}.
 Arguments pkg_functions (pkg_name) {_ _}.
 Arguments pkg_msets (pkg_name) {_ _}.
 Arguments pkg_imported_pkgs (pkg_name) {_ _}.
+
+Module option.
+Section defns.
+Context `{ffi_syntax}.
+
+Definition unwrap_def : val :=
+  λ: "x", match: "x" with
+            NONE => #() #()
+          | SOME "x" => "x"
+          end.
+Program Definition unwrap := sealed @unwrap_def.
+Definition unwrap_unseal : unwrap = _ := seal_eq _.
+
+End defns.
+End option.
+
+Module globals.
+Section defns.
+Context `{ffi_syntax}.
+
+Definition get_def : val :=
+  λ: "var_name", match: alist_lookup "var_name" (option.unwrap $ GlobalGet #"__global_vars") with
+                   NONE => #null
+                 | SOME "v" => "v"
+                 end .
+Program Definition get := sealed @get_def.
+Definition get_unseal : get = _ := seal_eq _.
+
+End defns.
+End globals.
+
+Module package.
+Section defns.
+Context `{ffi_syntax}.
+
+(* Allocates variables *just* for a single package. Unsealed because user proves
+   WPs for this by unfolding. *)
+Definition alloc pkg_name `{!PkgInfo pkg_name} : val :=
+  λ: <>, (fix alloc (vars : list (go_string * go_type)) : expr :=
+           (match vars with
+            | Datatypes.nil => #()
+            | (pair name t) :: vars =>
+                let: "addr" := mem.alloc (zero_val t) in
+                assume (globals.get #name = "addr")
+            end)%E) (pkg_vars pkg_name).
+
+Definition init_def (pkg_name : go_string) : val :=
+  λ: "init", match: GlobalGet #pkg_name with
+               SOME <> => #()
+             | NONE => "init" #()
+             end.
+Program Definition init := sealed @init_def.
+Definition init_unseal : init = _ := seal_eq _.
+End defns.
+End package.
+
+Section defns.
+Context `{ffi_syntax}.
+
+Definition func_call_def : val :=
+  λ: "func_name",
+    (λ: "firstArg",
+       (option.unwrap $ alist_lookup "func_name" (option.unwrap $ GlobalGet #"__functions")) "firstArg").
+Program Definition func_call := sealed @func_call_def.
+Definition func_call_unseal : func_call = _ := seal_eq _.
+
+Definition method_call_def : val :=
+  λ: "type_id" "method_name" "receiver",
+    λ: "firstArg",
+       let: "method_set" := option.unwrap $ alist_lookup "type_id" (option.unwrap $ GlobalGet #"__msets") in
+       (option.unwrap $ alist_lookup "method_name" "method_set") "receiver" "firstArg"
+    .
+Program Definition method_call := sealed @method_call_def.
+Definition method_call_unseal : method_call = _ := seal_eq _.
+
+End defns.
