new/golang/theory/pkg.v
@@ -1,8 +1,221 @@
 From Perennial.goose_lang Require Import notation.
-From New.golang.theory Require Import proofmode globals.
-From New.golang.defn Require Import globals pkg.
+From New.golang.theory Require Import exception mem typing list.
 From New.golang.defn Require Export pkg.
-Import Ltac2.
+From Perennial Require Import base.
+
+Set Default Proof Using "Type".
+
+Section wps.
+Context `{sem: ffi_semantics} `{!ffi_interp ffi} `{!heapGS Σ}.
+Global Instance wp_unwrap (v : val) :
+  PureWp True (option.unwrap $ InjRV v) v.
+Proof.
+  rewrite option.unwrap_unseal /option.unwrap_def.
+  intros ?????. iIntros "Hwp". wp_pure_lc "?".
+  wp_pures. by iApply "Hwp".
+Qed.
+End wps.
+
+(** [GoContext] contains the global state of a node running Go code. It is a
+    typeclass so that [global_addr] can be conveniently used in proofs that have
+    a section variable of type [GoContext]. A new [global_addr] is (angelically)
+    nondeterministically chosen on reboot. This choice is angelic in the sense
+    that future code (package.alloc) will actually allocate on the heap and
+    angelically assumes that the allocated location matches the [global_addr]
+    map.
+
+    TODO: not sure if having [is_pkg_init] makes sense in here. The other three
+    fields are directly related to execution state, but the [is_pkg_init]
+    consists of predicates chosen by the proof developer.
+ *)
+Class GoContext {ext : ffi_syntax} Σ :=
+  {
+    global_addr : go_string → loc;
+    is_pkg_init : go_string → iProp Σ;
+    __function : list (go_string * val);
+    __method : list (go_string * (list (go_string * val)));
+  }.
+
+Section globals.
+Context `{ffi_sem: ffi_semantics} `{!ffi_interp ffi} `{!heapGS Σ}.
+Context `{!GoContext Σ}.
+
+Definition is_go_context : iProp Σ :=
+    inv nroot (
+        ∃ (global_addr_val : list (_ * loc)) package_inited,
+        "Hg" ∷ own_globals 1 (
+            <["__global_vars"%go := alist_val ((λ '(a, b), (a, #b)) <$> global_addr_val)]>
+              (<["__functions"%go := alist_val __function]>
+                 (<["__msets"%go := alist_val ((λ '(a, b), (a, alist_val b)) <$> __method)]>
+                    package_inited))) ∗
+        "#Hinit" ∷ □([∗ map] pkg_name ↦ _ ∈ package_inited, is_pkg_init pkg_name) ∗
+        "%Hglobal_addr" ∷ ⌜ ∀ var_name, default null (alist_lookup_f var_name global_addr_val) = global_addr var_name ⌝
+      ).
+
+Lemma alist_lookup_f_fmap {A B} n (l: list (go_string * A)) (f : A → B) :
+  alist_lookup_f n ((λ '(name, a), (name, f a)) <$> l) =
+  f <$> (alist_lookup_f n l).
+Proof.
+  induction l as [|[]]; first done; simpl.
+  destruct (ByteString.eqb g n); first done.
+  rewrite IHl //.
+Qed.
+
+Definition func_callv_def (func_name : go_string) : func.t :=
+  {|
+    func.f := <>; func.x := "firstArg";
+    func.e :=
+      option.unwrap (alist_lookup (# func_name) (option.unwrap (GlobalGet (# "__functions"%go))))
+        "firstArg"
+  |}.
+Program Definition func_callv := sealed @func_callv_def.
+Definition func_callv_unseal : func_callv = _ := seal_eq _.
+
+Global Instance wp_func_callv (func_name : go_string) :
+  PureWp True (func_call #func_name)%E #(func_callv func_name)%E.
+Proof.
+  rewrite func_call_unseal /func_call_def func_callv_unseal.
+  intros ?????. iIntros "Hwp". wp_pure_lc "?".
+  wp_pures. by iApply "Hwp".
+Qed.
+
+Definition method_callv_def (type_name method_name : go_string) (receiver : val) : func.t :=
+  {|
+    func.f := <>; func.x := "firstArg";
+    func.e :=
+      let: "method_set" := option.unwrap
+                             (alist_lookup (# type_name) (option.unwrap (GlobalGet #"__msets"))) in
+      option.unwrap (alist_lookup (# method_name) "method_set") receiver "firstArg"
+  |}.
+
+Program Definition method_callv := sealed @method_callv_def.
+Definition method_callv_unseal : method_callv = _ := seal_eq _.
+
+Global Instance wp_method_callv (type_name method_name : go_string) (receiver : val) :
+  PureWp True (method_call #type_name #method_name receiver) #(method_callv type_name method_name receiver).
+Proof.
+  rewrite method_call_unseal /method_call_def method_callv_unseal.
+  intros ?????. iIntros "Hwp". wp_pure_lc "?".
+  wp_pures. by iApply "Hwp".
+Qed.
+
+(** Internal-ish to Goose. Users should never manually define instances of this.
+    The [P] predicate will generally be a package's [is_defined]. *)
+Class WpFuncCall func_name (f : val) (P : iProp Σ) :=
+  wp_func_call :
+    (∀ (first_arg : val) Φ,
+       P -∗ (WP (f first_arg) {{ Φ }}) -∗
+       WP #(func_callv func_name) first_arg {{ Φ }}).
+
+(** Same as [WpFuncCall]. *)
+Class WpMethodCall (type_name : go_string) (func_name : go_string) (m : val)
+                   (P : iProp Σ)
+  := wp_method_call :
+    (∀ (first_arg receiver : val) Φ,
+         P -∗ (WP (m receiver first_arg) {{ Φ }}) -∗
+         WP #(method_callv type_name func_name receiver) first_arg {{ Φ }}).
+
+(** This says that the package's declarations are accessible (including
+    functions, methods, and variables). *)
+Definition is_defined_def pkg_name `{!PkgInfo pkg_name} : iProp Σ :=
+  "#Hctx" ∷ is_go_context ∗
+  "%Hfunction" ∷ ⌜ (∀ func_name func,
+                      (alist_lookup_f func_name (pkg_functions pkg_name)) = Some func →
+                      (alist_lookup_f func_name __function) = Some func) ⌝ ∗
+  "%Hmethod" ∷ ⌜ (∀ type_name method_name m,
+                      (alist_lookup_f type_name (pkg_msets pkg_name)) ≫=
+                      (alist_lookup_f method_name) = Some m →
+                      (alist_lookup_f type_name __method) ≫=
+                      (alist_lookup_f method_name) = Some m) ⌝.
+Program Definition is_defined := sealed @is_defined_def.
+Definition is_defined_unseal : is_defined = _ := seal_eq _.
+#[global] Arguments is_defined (pkg_name) {_}.
+#[global] Instance is_defined_persistent pkg_name `{!PkgInfo pkg_name} : Persistent (is_defined pkg_name).
+Proof. rewrite is_defined_unseal. apply _. Qed.
+
+(** Any package's [is_defined] suffices as precondition. *)
+Lemma wp_globals_get pkg_name `{!PkgInfo pkg_name} var_name :
+  {{{ is_defined pkg_name }}} (globals.get #var_name) {{{ RET #(global_addr var_name); True }}}.
+Proof.
+  iIntros (?) "#Hdef HΦ". rewrite globals.get_unseal.
+  rewrite is_defined_unseal. iNamed "Hdef". clear Hfunction Hmethod PkgInfo0. iNamed "Hctx".
+  wp_call_lc "Hlc". wp_bind.
+  iInv "Hctx" as "Hi" "Hclose".
+  iMod (lc_fupd_elim_later with "[$] Hi") as "Hi". iNamed "Hi".
+  rewrite [in # "__global_vars"]to_val_unseal.
+  wp_apply (wp_GlobalGet with "[$]").
+  iIntros "Hg".
+  iMod ("Hclose" with "[Hg Hinit]").
+  { iFrame "∗#%". }
+  iModIntro.
+  rewrite lookup_insert_eq.
+  wp_pures. specialize (Hglobal_addr var_name).
+  rewrite alist_lookup_f_fmap.
+  destruct alist_lookup_f.
+  { simpl in *. subst. wp_pures. by iApply "HΦ". }
+  { simpl in *. wp_pures. rewrite <-Hglobal_addr. by iApply "HΦ". }
+Qed.
+
+(** Internal to Goose. Used in generatedproofs to establish [WpFuncCall]. *)
+Lemma wp_func_call' {func_name func} `{!PkgInfo pkg_name} :
+  alist_lookup_f func_name (pkg_functions pkg_name) = Some func →
+  WpFuncCall func_name func (is_defined pkg_name).
+Proof.
+  intros Hlookup. rewrite /WpFuncCall. iIntros "* Hdef HΦ". rewrite func_callv_unseal.
+  wp_pure_lc "Hlc". wp_bind. iNamed "Hdef". rewrite is_defined_unseal.
+  iNamed "Hdef". iInv "Hctx" as "Hi" "Hclose". iMod (lc_fupd_elim_later with "[$] Hi") as "Hi".
+  iNamed "Hi". rewrite [in # "__functions"]to_val_unseal. wp_apply (wp_GlobalGet with "[$]").
+  iIntros "Hg". iMod ("Hclose" with "[Hg Hinit]"). { iFrame "∗#%". }
+  iModIntro. rewrite lookup_insert_ne // lookup_insert_eq.
+  wp_pures. erewrite Hfunction; last done. wp_pures. iApply "HΦ".
+Qed.
+
+(** Internal to Goose. Used in generatedproofs to establish [WpMethodCall]. *)
+Lemma wp_method_call' {type_name method_name m} `{!PkgInfo pkg_name} :
+  (alist_lookup_f type_name (pkg_msets pkg_name)) ≫= (alist_lookup_f method_name) = (Some m) →
+  WpMethodCall type_name method_name m (is_defined pkg_name).
+Proof.
+  intros Hlookup. rewrite /WpMethodCall. iIntros "* Hdef HΦ". rewrite method_callv_unseal.
+  wp_pure_lc "Hlc". wp_bind. iNamed "Hdef". rewrite is_defined_unseal.
+  iNamed "Hdef". iInv "Hctx" as "Hi" "Hclose". iMod (lc_fupd_elim_later with "[$] Hi") as "Hi".
+  iNamed "Hi". rewrite [in # "__msets"]to_val_unseal. wp_apply (wp_GlobalGet with "[$]").
+  iIntros "Hg". iMod ("Hclose" with "[Hg Hinit]"). { iFrame "∗#%". }
+  iModIntro. do 2 rewrite lookup_insert_ne //. rewrite lookup_insert_eq.
+  wp_pures. rewrite alist_lookup_f_fmap. specialize (Hmethod _ _ _ Hlookup).
+  destruct (alist_lookup_f type_name __method); last by exfalso.
+  wp_pures. simpl in *. destruct (alist_lookup_f method_name l); last by exfalso.
+  wp_pures. simplify_eq. iApply "HΦ".
+Qed.
+
+End globals.
+
+Global Hint Mode WpMethodCall - - - - - - + + - - : typeclass_instances.
+Global Hint Mode WpFuncCall - - - - - - + - - : typeclass_instances.
+
+(* TODO: better error messages if tc_solve fails to find a val for the name. *)
+Tactic Notation "wp_globals_get_core" :=
+  wp_bind (globals.get _ _);
+  unshelve iApply (wp_globals_get with "[]").
+
+Tactic Notation "wp_func_call_core" :=
+  (wp_bind (#(func_callv _ _) _);
+   unshelve iApply (wp_func_call with "[]");
+   [| | (tc_solve || fail "could not find mapping from function name to val") | | ]).
+
+Tactic Notation "wp_method_call_core" :=
+  (wp_bind (#(method_callv _ _ _ _) _);
+   unshelve iApply (wp_method_call with "[]");
+   [| | (tc_solve || fail "could not find mapping from method to val") | |]).
+
+#[global]
+Notation "pkg @ func" :=
+  #(func_callv pkg func) (at level 1, no associativity) : expr_scope.
+
+#[global]
+Notation "rcvr @ pkg @ type @ method" :=
+  #(method_callv pkg type method #rcvr)
+    (at level 1, pkg at next level, type at next level, no associativity) : expr_scope.
+
 
 (** [IsPkgInit] is used to record a mapping from pkg names to an
 initialization predicate, which is the postcondition for after the package has
@@ -19,7 +232,8 @@ incomparable ones.
 *)
 Class IsPkgInit (pkg_name: go_string) {PROP: bi} :=
   {
-    is_pkg_init_def : PROP ;
+    is_pkg_init_def : PROP ; (* user-specified *)
+    is_pkg_init_deps : PROP ; (* autogenerated *)
     #[global]
     is_pkg_init_persistent :: Persistent is_pkg_init_def;
   }.
@@ -29,10 +243,15 @@ Arguments is_pkg_init_def (pkg_name) {_ _}.
 #[global]
 Typeclasses Opaque is_pkg_init_def.
 
-(* XXX: To avoid printing the IsPkgInit instances when printing [is_pkg_init]
-   See https://github.com/coq/coq/issues/9814 for a description of the problem. *)
-#[global]
-Notation is_pkg_init := is_pkg_init_def.
+Section is_pkg_init.
+Context `{ffi_sem: ffi_semantics} `{!ffi_interp ffi} `{!heapGS Σ}.
+Context `{!GoContext Σ}.
+Definition is_pkg_init_aux `{!PkgInfo pkg_name} `{!IsPkgInit pkg_name} : iProp Σ :=
+  "#Hdefined" ∷ is_defined pkg_name ∗
+  "#Hdeps" ∷ □ is_pkg_init_deps ∗
+  "#Hinit" ∷ is_pkg_init_def pkg_name.
+
+End is_pkg_init.
 
 #[global]
 Hint Mode IsPkgInit + - : typeclass_instances.
@@ -40,24 +259,7 @@ Hint Mode IsPkgInit + - : typeclass_instances.
 Ltac prove_is_pkg_init :=
   constructor; refine _.
 
-(** [IsPkgDefined] is analogous to [IsPkgInit] but looks up the
-    post-definition predicate. This is something that can be auto-generated. *)
-Class IsPkgDefined (pkg_name: go_string) {PROP: bi} :=
-  {
-    is_pkg_defined_def : PROP;
-    #[global]
-    is_pkg_defined_persistent :: Persistent is_pkg_defined_def;
-  }.
-
-#[global]
-Arguments is_pkg_defined_def (pkg_name) {_ _}.
-
-#[global]
-Notation is_pkg_defined := is_pkg_defined_def.
-
-#[global]
-Hint Mode IsPkgDefined + - : typeclass_instances.
-
+Import Ltac2.
 Ltac2 build_pkg_init () :=
   Control.refine
     (fun () =>
@@ -69,7 +271,7 @@ Ltac2 build_pkg_init () :=
              | cons ?pkg ?deps =>
                  let rest := build_iprop deps in
                  constr:((is_pkg_init $pkg ∗ $rest)%I)
-             | nil => constr:(is_pkg_defined_def $name)
+             | nil => constr:(is_defined_def $name)
              | _ =>
                  Message.print (Message.of_constr deps);
                  Control.backtrack_tactic_failure "build_pkg_init: unable to match deps list"
@@ -87,8 +289,8 @@ Ltac solve_pkg_init :=
   unfold named;
   lazymatch goal with
   | |- environments.envs_entails ?env (is_pkg_init _) => idtac
-  | |- environments.envs_entails ?env (is_pkg_defined _) => idtac
-  | _ => fail "not a is_pkg_init or is_pkg_defined goal"
+  | |- environments.envs_entails ?env (is_defined _) => idtac
+  | _ => fail "not a is_pkg_init or is_defined goal"
   end;
   iClear "∗";
   simpl is_pkg_init;
